---
index: 2
caption: Fanning Out
statement: |
    Suppose random variables X and Y have joint density given by,

    $$f(x,y) = \begin{cases} 1/x, &0 < x < 1, 0 < y < x \\\\\
    0, &otherwise
    \end{cases}
    $$

    This is a long (but revealing) way to compute $V[Y]$

    1. Compute the marginal distribution of X.
    2. Compute $V[Y\|X]$.  This will be a fuction of X.
    3. Compute $E[ V[Y\|X]]$.  This will be a number.
    4. Compute $E[Y\|X]$.  This will be a function of X.
    5. Compute $V[ E[Y\|X]]$.  This will be a number.
    6. Using the law of total variance, compute $V[Y]$.
---
1. Compute the marginal distribution of X

$$f(x) = \int_{0}^{x} \frac{1}{x} \, dx = \left. \frac{y}{x} \right|_{0}^{x} = 1
$$
$$\rightarrow f(x) = \begin{cases} 1, &0 < x < 1\\\\\
0, &otherwise
\end{cases}
$$  

2. To obtain $V(Y\mid X)$
We need $E[Y^2\mid X]$ and $E[Y\mid X]$ because $V(Y\mid X)$ = $E[Y^2\mid X]$ + $(E[Y\mid X])^2$
So we first need to find $f(y\mid x) = $

$$f(y \mid x) = \frac{f(x, y)}{f(x)} = \frac{\frac{1}{x}}{1} = \frac{1}{x}= \begin{cases} 1, &0 < y < x\\\\\
0, &otherwise
\end{cases}
$$
So ... 
$$ E[Y\mid X] =  = \int_{0}^{x} y \frac{1}{x} \, dx = \left. \frac{y^2}{2x} \right|_{0}^{x} = \frac{x}{2}$$
and by LOTUS
$$ E[Y^2\mid X] =  \int_{0}^{x} y^2 \frac{1}{x} \, dx = \left. \frac{y^3}{3x} \right|_{0}^{x} = \frac{x^2}{3}$$
Putting together the terms for $V(Y \mid X)$ we have
$$\frac{x^2}{3} - \frac{x^2}{4} = \frac{x^2}{12}  \text{, for }  0<x<1$$

3. The $E[V(Y\mid X)] = E[\frac{x^2}{12}] = $ (by LOTUS)
$$\int_{0}^{1} \frac{x^2}{12} \frac{1}{x} \, dx = \int_{0}^{1} \frac{x}{12} \, dx = \left. \frac{x^2}{24} \right|_{0}^{1} = \frac{1}{24}$$

4. The $E[Y\mid X]$ we have from before as $\frac{x}{2}$.

5. The $V(E[Y \mid X]) = $  (by definition)
$$E[(E[Y \mid X])^2] - (E[E[Y \mid X]])^2 =$$

from previous result 
$$ E[\frac{X^2}{4}] - (E[\frac{X}{2}])^2$$

3. The $E[V(Y\mid X)] = E[\frac{x^2}{12}] = $ (by LOTUS)
$$\int_{0}^{1} \frac{x^2}{12} \frac{1}{x} \, dx = \int_{0}^{1} \frac{x}{12} \, dx = \left. \frac{x^2}{24} \right|_{0}^{1} = \frac{1}{24}$$
4. The $E[Y\mid X]$ we have from before as $\frac{x}{2}$.

5. The $V(E[Y \mid X]) = $  (by definition)
$$E[(E[Y \mid X])^2] - (E[E[Y \mid X]])^2 =$$

from previous result 
$$ E[\frac{X^2}{4}] - (E[\frac{X}{2}])^2$$

For $E[\frac{X^2}{4}] = $ (by LOTUS)
$$\int_{0}^{1} \frac{x^2}{4} *1 \text{ } dx = \int_{0}^{1} \frac{x^2}{4} \, dx = \left. \frac{x^3}{12} \right|_{0}^{1} = \frac{1}{12}$$

and also by LOTUS 
$$E[\frac{x}{2}] = \int_{0}^{1} \frac{x}{2} *1 \text{ } dx = \left. \frac{x^2}{4} \right|_{0}^{1} = \frac{1}{4}$$
$$\rightarrow (E[\frac{x}{2}])^2 = \frac{1}{16}$$

$$\rightarrow V(E[Y \mid X]) = \frac{1}{12} - \frac{1}{16} = \frac{1}{48}$$

6. Finally by the Law of Total Variance or EVE's Law (coming from the mnemonic EV+VE)  $V(Y) =$
$$E[V(Y\mid X)] + V(E[Y \mid X]) = \frac{1}{24} + \frac{1}{48} = \frac{1}{16}$$
