---
index: 6
statement: |
    Using the clues given below, fill in the rest of the joint distribution. There is only one answer:

    |$Y$|$X=1$|2|3|
    |$1$|$?$|$?$|$?$|
    |$2$|$?$|$0$|$?$|
    |$3$|$0$|$?$|$0$|

    For $k=1, 2, 3$, (a) $P(Y=1\|X=k)=\frac{2}{3}$, 
    (b) $P(X=k\|Y=1)=\frac{k}{6}$.
---
Let us assume the following probabilities:

 |$Y$|$X=1$|2|3|
 |$1$|$p_1$|$p_2$|$p_3$|
 |$2$|$p_4$|$0$|$p_5$|
 |$3$|$0$|$p_6$|$0$|
 
 From the fact that the sum of all entries is $1$, we have that 
 $$p_1+p_2+p_3+p_4+p_5+p_6=1.$$
 
 **Using (a)**   
 for $k=1$, $$\frac{p_1}{p_1+p_4}=\frac{2}{3}\implies p_1=2p_4$$  
 for $k=2$, $$\frac{p_2}{p_2+p_6}=\frac{2}{3}\implies p_2=2p_6$$  
 for $k=3$, $$\frac{p_3}{p_3+p_5}=\frac{2}{3}\implies p_3=2p_5$$  

So, 
$$p_1+p_2+p_3=2(p_4+p_5+p_6)=2(1-p_1-p_2-p_3)\implies p_1+p_2+p_3=\frac{2}{3}.$$

 **Using (b)**   
 for $k=1$, $$\frac{p_1}{p_1+p_2+p_3}=\frac{1}{6}\implies p_1=\frac{1}{6}(p_1+p_2+p_3)=\frac{1}{9}$$  
 for $k=2$, $$\frac{p_2}{p_1+p_2+p_3}=\frac{2}{6}\implies p_2=\frac{2}{6}(p_1+p_2+p_3)=\frac{2}{9}$$  
 for $k=3$, $$\frac{p_3}{p_1+p_2+p_3}=\frac{3}{6}\implies p_3=\frac{3}{6}(p_1+p_2+p_3)=\frac{3}{9}$$  
 
 Also, $$p_4=\frac{1}{18},p_5=\frac{3}{18},p_6=\frac{2}{18}.$$
 