---
index: 2
level: 0
statement: |
    Prove Bonferroni's inequality:  
    $$P(A\cap B)\geq P(A) + P(B) - 1.$$
    Hint: The addition rule and Kolmogorov's axioms.
---
Hint: The addition rule and Kolmogorov's axioms.

\\[
    \begin{align}
    \text{Restate & Bonferroni's inequality}\\\\\
    P(A\cap B) &\geq P(A) + P(B) - 1
    \\\\\
    \text{Addition Rule &Thrm 1.1.7}\\\\\
    P(A\cup B) &= P(A) + P(B) - P(A\cap B)\\\\\
    0 &= P(A) + P(B) - P(A\cap B) - P(A\cup B) \\\\\
    P(A\cap B) &= P(A) + P(B) - P(A\cup B)
    \\\\\
    \text{Plug in to & Bonferroni's inequality}\\\\\
    P(A) + P(B) - P(A\cup B) &\geq P(A) + P(B) - 1\\\\\
                - P(A\cup B) &\geq (-1) \\\\\
                  P(A\cup B) &\leq 1\\\\\
    \end{align}
\\]

From Thrm 1.1.4 basic properties of probability (probability bounds),
we know that the statement $P(A\cup B) \leq 1$ is true. Therefore the
supposition that led to it is also true. We have proven Bonferroni's 
inequality.

(_For those keeping score, the Kolgomorov axioms (Defn 1.1.2) come into
this because they are the direct source of our basic properties of 
probability presented in Thrm 1.1.4_)
