---
index: 2
level: 2
caption: Recursive Conditional
statement: |
    Suppose there are $n$ events, $A_1,A_2,...,A_n$ and the intersection of all these events is non-empty. Write an inductive proof to show that
    $$P(A_1\cap A_2\cap\ldots \cap A_n)=P(A_1)P(A_2|A_1)P(A_3|A_1\cap A_2)\ldots P(A_n|A_1\cap A_2\cap\ldots\cap A_{n-1}).$$
---
For $n=1$, we have the trivial statement that $P(A_1)=P(A_1)$.
Now let's assume that the statement whenever $n < N$. In particular, it is true when n = N-1, i.e.:

$$P(A_1,A_2,...,A_{N-1})=P(A_1)P(A_2|A_1)...P(A_{N-1}|A_1\cap A_2\cap ... \cap A_{N-2})$$

To show the statement holds for $n=N$, let's define an event B, where: 

$B=A_1\cap A_2 \cap ... \cap A_{N-1}$

$$  P(A_1,A_2,...,A_{N-1},A_n)=P(B \cap A_N)$$

From Bayes rule we have:

$$P(B \cap A_N)=P(B)P(A_N|B)$$


Substituting $A_1\cap A_2 \cap ... \cap A_{N-1}$ for B, and equation (1), we have our proof:

$$ P(A_1\cap A_2 \cap ... \cap A_{N-1} \cap A_N)=P(A_1\cap A_2 \cap ... \cap A_{N-1})P(A_N|A_1\cap A_2 \cap ... \cap A_{N-1}) $$

$$\begin{align*}
P(A_1\cap A_2 \cap ... \cap A_{N-1} \cap A_N)= \\
     P(A_1)P(A_2|A_1)...P(A_{N-1}|A_1\cap A_2\cap ... \cap A_{N-2})P(A_N|A_1\cap A_2 \cap ... \cap A_{N-1}) 
\end{align*}$$
